fix Decimal.unParse
Signed-off-by: Craig Disselkoen <cdiss@amazon.com>

cedar-lean/Cedar/Spec/Ext/Decimal.lean
@@ -59,9 +59,26 @@ def parse (str : String) : Option Decimal :=
   | _ => .none
 
 def unParse (d : Decimal) : String :=
-  let left  := d / (Int.pow 10 DECIMAL_DIGITS)
-  let right := d % (Int.pow 10 DECIMAL_DIGITS)
-  ToString.toString left ++ "." ++ ToString.toString right
+  let neg   := d < (0 : Int)
+  let d     := d.natAbs
+  let left  := d / (Nat.pow 10 DECIMAL_DIGITS)
+  let right := d % (Nat.pow 10 DECIMAL_DIGITS)
+  let right :=
+    -- this is not generalized for arbitrary DECIMAL_DIGITS
+    if right < 10 then ".000" ++ ToString.toString right
+    else if right < 100 then ".00" ++ ToString.toString right
+    else if right < 1000 then ".0" ++ ToString.toString right
+    else "." ++ ToString.toString right
+  (if neg then "-" else "") ++ ToString.toString left ++ right
+
+theorem test1 : unParse ((parse "3.14").get!) = "3.1400" := by decide
+theorem test2 : unParse ((parse "11.0003").get!) = "11.0003" := by decide
+theorem test3 : unParse ((parse "11.003").get!) = "11.0030" := by decide
+theorem test4 : unParse ((parse "11.3000").get!) = "11.3000" := by decide
+theorem test5 : unParse ((parse "123.0").get!) = "123.0000" := by decide
+theorem test6 : unParse ((parse "-123.0").get!) = "-123.0000" := by decide
+theorem test7 : unParse ((parse "-3.14").get!) = "-3.1400" := by decide
+theorem test8 : unParse ((parse "-11.0003").get!) = "-11.0003" := by decide
 
 abbrev decimal := parse
 
